src/proof/apimodel.v
@@ -58,52 +58,11 @@ Definition extract_kobject_metadata kobj : v1.ObjectMeta.t :=
 Definition mk_replicaset_key (namespace name: go_string) : KKey.t :=
   {| KKey.Kind' := "ReplicaSet"%go; KKey.Namespace' := namespace; KKey.Name' := name;|}.
 
-Definition pod_rep k v1 v2 ptr pod : iProp Σ :=
-  "%interface_is_pod_ptr" ∷ ⌜ v1 = interface.mk (ptrT.id v1.Pod.id) #ptr ⌝ ∗
-  "pod_ptr" ∷ ptr ↦ pod ∗
-  "%abs_v_is_pod" ∷ ⌜ v2 = KObject.Pod pod ⌝ ∗
-  "pod_nn_well_formed" ∷ pod_nn_well_formed pod (KKey.Namespace' k) (KKey.Name' k).
+Definition has_controller_parent (oslice: slice.t) (os: list v1.OwnerReference.t) (o: v1.OwnerReference.t) (c: bool) : iProp Σ :=
+  oslice ↦* os ∗ ⌜ o ∈ os ⌝ ∗ o.(v1.OwnerReference.Controller') ↦ c ∗ ⌜ c = true ⌝.
 
-Definition replicaset_rep k v1 v2 ptr rs : iProp Σ :=
-  "%interface_is_rs_ptr" ∷ ⌜ v1 = interface.mk (ptrT.id v1.ReplicaSet.id) #ptr ⌝ ∗
-  "rs_ptr" ∷ ptr ↦ rs ∗
-  "%abs_v_is_rs" ∷ ⌜ v2 = KObject.ReplicaSet rs ⌝ ∗
-  "replicaset_nn_well_formed" ∷ replicaset_nn_well_formed rs (KKey.Namespace' k) (KKey.Name' k).
-
-Definition state_rep (phys_state: gmap KKey.t interface.t) (abs_state: gmap KKey.t KObject.t) : iProp Σ :=
-  [∗ map] k ↦ v1; v2 ∈ phys_state; abs_state,
-    if bool_decide (KKey.Kind' k = "Pod"%go) then
-      ∃ (ptr: loc) (pod: v1.Pod.t), pod_rep k v1 v2 ptr pod
-    else if bool_decide (KKey.Kind' k = "ReplicaSet"%go) then
-      ∃ (ptr: loc) (rs: v1.ReplicaSet.t), replicaset_rep k v1 v2 ptr rs
-    else False%I.
-
-Axiom kubernetes_state_consistent: gmap KKey.t KObject.t → gmap KKey.t (gset KKey.t) → gset KKey.t → iProp Σ. 
-
-Definition is_kubernetes_state_inner γ_state γ_children γ_fresh_keys: iProp Σ :=
-  ∃ (l: loc) (uc: w64) (rvc: w64) (phys_state: gmap KKey.t interface.t) (abs_state: gmap KKey.t KObject.t) (children: gmap KKey.t (gset KKey.t)) (fresh_keys: gset KKey.t),
-    "state_m_addr" ∷ (global_addr apimodel.state) ↦s[ apimodel.State :: "m" ] l ∗
-    "state_uc_addr" ∷ (global_addr apimodel.state) ↦s[ apimodel.State :: "uidCounter" ] uc ∗
-    "state_rvc_addr" ∷ (global_addr apimodel.state) ↦s[ apimodel.State :: "resourceVersionCounter" ] rvc ∗
-    "own_phys" ∷ l ↦$ phys_state ∗
-    "own_abs" ∷ map_ctx γ_state 1 abs_state ∗
-    "phys_abs_rep" ∷ state_rep phys_state abs_state ∗
-    "own_children" ∷ map_ctx γ_children 1 children ∗
-    "own_fresh_keys" ∷ auth_set_auth γ_fresh_keys fresh_keys ∗
-    "consistent" ∷ kubernetes_state_consistent abs_state children fresh_keys.
-
-Definition is_kubernetes_state γ_state γ_children γ_fresh_keys : iProp Σ :=
-  is_Mutex (global_addr apimodel.stateMu) (is_kubernetes_state_inner γ_state γ_children γ_fresh_keys).
-
-Definition pod_has_controller_parent_uid (pod: v1.Pod.t) (os: list v1.OwnerReference.t) (o: v1.OwnerReference.t) (c: bool) : iProp Σ :=
-  pod.(v1.Pod.ObjectMeta').(v1.ObjectMeta.OwnerReferences') ↦* os ∗
-  ⌜ o ∈ os ⌝ ∗
-  o.(v1.OwnerReference.Controller') ↦ c ∗
-  ⌜ c = true ⌝.
-
-Definition is_pod_controller_uid_index (pod: v1.Pod.t) (indexed_value: go_string) : iProp Σ :=
-  (∃ os o c, pod_has_controller_parent_uid pod os o c ∗ ⌜ o.(v1.OwnerReference.UID') = indexed_value ⌝) ∨
-  (¬(∃ os o c, pod_has_controller_parent_uid pod os o c) ∗ ⌜ indexed_value = "_ORPHAN_POD"%go ⌝).
+Definition has_controller_parent_of (oslice: slice.t) (uid: go_string) : iProp Σ :=
+  ∃ os o c, has_controller_parent oslice os o c ∗ ⌜ o.(v1.OwnerReference.UID') = uid ⌝.
 
 Lemma decide_kind_is_pod kind:
   kind = "Pod"%go →
@@ -126,6 +85,68 @@ Proof.
   - apply bool_decide_true; exact Hkind.
   - apply bool_decide_false. intros Hcontra. rewrite Hcontra in Hkind. done.
 Qed.
+
+Definition pod_rep k v1 v2 ptr pod : iProp Σ :=
+  "%interface_is_pod_ptr" ∷ ⌜ v1 = interface.mk (ptrT.id v1.Pod.id) #ptr ⌝ ∗
+  "pod_ptr" ∷ ptr ↦ pod ∗
+  "%abs_v_is_pod" ∷ ⌜ v2 = KObject.Pod pod ⌝ ∗
+  "pod_nn_well_formed" ∷ pod_nn_well_formed pod (KKey.Namespace' k) (KKey.Name' k).
+
+Definition replicaset_rep k v1 v2 ptr rs : iProp Σ :=
+  "%interface_is_rs_ptr" ∷ ⌜ v1 = interface.mk (ptrT.id v1.ReplicaSet.id) #ptr ⌝ ∗
+  "rs_ptr" ∷ ptr ↦ rs ∗
+  "%abs_v_is_rs" ∷ ⌜ v2 = KObject.ReplicaSet rs ⌝ ∗
+  "replicaset_nn_well_formed" ∷ replicaset_nn_well_formed rs (KKey.Namespace' k) (KKey.Name' k).
+
+Definition obj_rep k v1 v2 : iProp Σ :=
+  (if bool_decide (KKey.Kind' k = "Pod"%go) then
+    ∃ (ptr: loc) (pod: v1.Pod.t), pod_rep k v1 v2 ptr pod
+  else if bool_decide (KKey.Kind' k = "ReplicaSet"%go) then
+    ∃ (ptr: loc) (rs: v1.ReplicaSet.t), replicaset_rep k v1 v2 ptr rs
+  else False)%I.
+
+Definition state_rep (phys_state: gmap KKey.t interface.t) (abs_state: gmap KKey.t KObject.t) : iProp Σ :=
+  [∗ map] k ↦ v1; v2 ∈ phys_state; abs_state, obj_rep k v1 v2.
+
+Definition kubernetes_state_consistent (abs_state: gmap KKey.t KObject.t) (children: gmap KKey.t (gset KKey.t)) (fresh_keys: gset KKey.t) : iProp Σ :=
+  (* All parents exist; this means holding a children gmap fragment implies the parent exists in abs_state *)
+  "%parents_exist" ∷ ⌜ dom children ⊆ dom abs_state ⌝ ∗
+  (* All children exist *)
+  "%children_exist" ∷ ⌜ ∀ k s, children !! k = Some s → s ⊆ dom abs_state ⌝ ∗
+  (* parents and children live in the same namespace *)
+  "%parents_children_same_namespace" ∷ ⌜ ∀ k s child_key, children !! k = Some s → child_key ∈ s → k.(KKey.Namespace') = child_key.(KKey.Namespace') ⌝ ∗
+  (* No one can be their own parent *)
+  "%no_self_parenting" ∷ ⌜ ∀ k s child_key, children !! k = Some s → child_key ∈ s → child_key ≠ k ⌝ ∗
+  (* Each children has only one parent -- the children gsets are disjoint *)
+  "%children_disjoint" ∷ ⌜ ∀ k1 s1 k2 s2, children !! k1 = Some s1 → children !! k2 = Some s2 → s1 ## s2 ⌝ ∗
+  (* Fresh keys are not used by any existing object *)
+  "%fresh_keys_absent" ∷ ⌜ fresh_keys ## dom abs_state ⌝ ∗
+  (* All of the children have the controller owner reference pointing to the parent's uid *)
+  "children_point_to_parent" ∷ (∀ k s parent child_key child,
+    ⌜ children !! k = Some s ∧ abs_state !! child_key = Some child ∧ abs_state !! k = Some parent ∧ child_key ∈ s⌝ -∗
+      has_controller_parent_of (extract_kobject_metadata child).(v1.ObjectMeta.OwnerReferences') (extract_kobject_metadata parent).(v1.ObjectMeta.UID')
+  ) ∗
+  (* Only the children have the controller owner reference pointing to the parent's uid *)
+  "only_children_point_to_parent" ∷ (∀ k s parent child_key child,
+    ⌜ children !! k = Some s ∧ abs_state !! child_key = Some child ∧ abs_state !! k = Some parent ⌝ ∗
+    has_controller_parent_of (extract_kobject_metadata child).(v1.ObjectMeta.OwnerReferences') (extract_kobject_metadata parent).(v1.ObjectMeta.UID') -∗
+      ⌜ child_key ∈ s ⌝
+  ).
+
+Definition is_kubernetes_state_inner γ_state γ_children γ_fresh_keys: iProp Σ :=
+  ∃ (l: loc) (uc: w64) (rvc: w64) (phys_state: gmap KKey.t interface.t) (abs_state: gmap KKey.t KObject.t) (children: gmap KKey.t (gset KKey.t)) (fresh_keys: gset KKey.t),
+    "state_m_addr" ∷ (global_addr apimodel.state) ↦s[ apimodel.State :: "m" ] l ∗
+    "state_uc_addr" ∷ (global_addr apimodel.state) ↦s[ apimodel.State :: "uidCounter" ] uc ∗
+    "state_rvc_addr" ∷ (global_addr apimodel.state) ↦s[ apimodel.State :: "resourceVersionCounter" ] rvc ∗
+    "own_phys" ∷ l ↦$ phys_state ∗
+    "own_abs" ∷ map_ctx γ_state 1 abs_state ∗
+    "phys_abs_rep" ∷ state_rep phys_state abs_state ∗
+    "own_children" ∷ map_ctx γ_children 1 children ∗
+    "own_fresh_keys" ∷ auth_set_auth γ_fresh_keys fresh_keys ∗
+    "consistent" ∷ kubernetes_state_consistent abs_state children fresh_keys.
+
+Definition is_kubernetes_state γ_state γ_children γ_fresh_keys : iProp Σ :=
+  is_Mutex (global_addr apimodel.stateMu) (is_kubernetes_state_inner γ_state γ_children γ_fresh_keys).
 
 Lemma wp_deepCopy_replicaset (obj: interface.t) (ptr: loc) (rs: v1.ReplicaSet.t):
   {{{ is_pkg_init apimodel ∗
@@ -193,7 +214,10 @@ Lemma wp_podControllerUIDIndex_with_controller_parent obj ptr pod:
       ⌜ err = interface.nil ⌝ ∗
       indexed_values ↦* indexed_value_list ∗
       ⌜ indexed_value_list = [indexed_value] ⌝ ∗
-      is_pod_controller_uid_index pod indexed_value
+      (
+        has_controller_parent_of pod.(v1.Pod.ObjectMeta').(v1.ObjectMeta.OwnerReferences') indexed_value ∨
+        (¬(∃ os o c, has_controller_parent pod.(v1.Pod.ObjectMeta').(v1.ObjectMeta.OwnerReferences') os o c) ∗ ⌜ indexed_value = "_ORPHAN_POD"%go ⌝)
+      )
   }}}.
 Proof.
 Admitted.
@@ -248,7 +272,7 @@ Lemma wp_ByIndex_pod_ptsto_mut kind index_name indexed_value
       ) ∗
       "pods_well_formed" ∷ ([∗ list] pod ∈ pods,
         pod_well_formed pod ∗
-        (∃ os o c, pod_has_controller_parent_uid pod os o c ∗ ⌜ o.(v1.OwnerReference.UID') = indexed_value ⌝)
+        has_controller_parent_of pod.(v1.Pod.ObjectMeta').(v1.ObjectMeta.OwnerReferences') indexed_value
       ) ∗
       "pods_found_in_map" ∷ ([∗ list] pod ∈ pods, ∃ owned_pod,
         ⌜ owned_pod_map !! extract_pod_key pod = Some owned_pod ⌝ ∗ deepcopy_Pod owned_pod pod
@@ -269,8 +293,7 @@ Lemma wp_PodCreate_without_name namespace to_create_pod_ptr to_create_pod
       "own_child_keys" ∷ parent_key [[ γ_children ]]↦ owned_child_keys ∗
       "%namespace_valid" ∷ ⌜ namespace = parent_key.(KKey.Namespace') ⌝ ∗
       "to_create_pod_ptr" ∷ to_create_pod_ptr ↦ to_create_pod ∗
-      "parent_uid" ∷ (∃ os o c, pod_has_controller_parent_uid to_create_pod os o c ∗
-        ⌜ o.(v1.OwnerReference.UID') = (extract_kobject_metadata owned_parent).(v1.ObjectMeta.UID') ⌝) ∗
+      "parent_uid" ∷ has_controller_parent_of to_create_pod.(v1.Pod.ObjectMeta').(v1.ObjectMeta.OwnerReferences') (extract_kobject_metadata owned_parent).(v1.ObjectMeta.UID') ∗
       "%no_name" ∷ ⌜ to_create_pod.(v1.Pod.ObjectMeta').(v1.ObjectMeta.Name') = ""%go ⌝ ∗
       "%generate_name" ∷ ⌜ to_create_pod.(v1.Pod.ObjectMeta').(v1.ObjectMeta.Name') ≠ ""%go⌝ ∗
       "well_formed_for_creation" ∷ pod_well_formed_for_creation to_create_pod
@@ -290,15 +313,6 @@ Lemma wp_PodCreate_without_name namespace to_create_pod_ptr to_create_pod
 Proof.
 Admitted.
 
-(* FIXME: this spec is wrong because o's value should be a Pod pointer. will fix it after Goose has better support for
-  interface method dispatch *)
-Lemma pod_ptr_implements_v1_object i (ptr: loc):
-  i = interface.mk (ptrT.id v1.Pod.id) (# ptr) →
-    ∃ (o: v1.Object.t), i = interface.mk v1.Object.id (# o) ∧
-      o = interface.mk (ptrT.id v1.ObjectMeta.id) #(struct.field_ref_f v1.Pod "ObjectMeta" ptr).
-Proof.
-Admitted.
-
 Lemma wp_FormatInt (i: w64) (base: w64):
   {{{ is_pkg_init apimodel }}}
     @! strconv.FormatInt #i #base
@@ -306,23 +320,33 @@ Lemma wp_FormatInt (i: w64) (base: w64):
 Proof.
 Admitted.
 
-Lemma wp_objDelete_ptsto_mut key γ_state γ_children γ_fresh_keys owned_pod parent_key owned_child_keys:
+(* If pod has a huge body, this lemma can be used to name the pod body *)
+Lemma rename_pod ptr (pod: v1.Pod.t):
+  ptr ↦ pod -∗ ∃ pod', ptr ↦ pod' ∗ ⌜ pod' = pod ⌝.
+Proof.
+  iIntros. iExists pod. iFrame. done.
+Qed.
+
+Lemma wp_objDelete_ptsto_mut key
+  γ_state γ_children γ_fresh_keys owned_pod parent_key owned_child_keys owned_grandchild_keys:
   {{{ is_pkg_init apimodel ∗
       "#inv" ∷ is_kubernetes_state γ_state γ_children γ_fresh_keys ∗
       "own_pod" ∷ key [[ γ_state ]]↦ (KObject.Pod owned_pod) ∗
       "own_child_keys" ∷ parent_key [[ γ_children ]]↦ owned_child_keys ∗
+      "own_grandchild_keys" ∷ key [[ γ_children ]]↦ owned_grandchild_keys ∗
       "%pod_is_child" ∷ ⌜ key ∈ owned_child_keys ⌝ ∗
       "%kind" ∷ ⌜ KKey.Kind' key = "Pod"%go ⌝
   }}}
     @! apimodel.objDelete #key
   {{{ (err: error.t) pod, RET #err;
       ⌜ err = interface.nil ⌝ ∗
-      (
+      ((
         key [[ γ_state ]]↦ (KObject.Pod pod) ∗
         parent_key [[ γ_children ]]↦ owned_child_keys ∗
+        key [[ γ_children ]]↦ owned_grandchild_keys ∗
         ⌜ pod.(v1.Pod.ObjectMeta').(v1.ObjectMeta.DeletionTimestamp') ≠ null ⌝
       ) ∨
-      parent_key [[ γ_children ]]↦ (owned_child_keys ∖ {[key]})
+      parent_key [[ γ_children ]]↦ (owned_child_keys ∖ {[key]}))
   }}}.
 Proof.
   wp_start as "H". iNamed "H".
@@ -333,10 +357,11 @@ Proof.
   iIntros "[own_Mutex H]". iNamed "H". wp_auto.
   wp_apply wp_globals_get. wp_apply wp_globals_get.
   iAssert (⌜ abs_state !! key = Some (KObject.Pod owned_pod) ⌝%I) with "[own_pod own_abs]" as "%key_in_abs".
-  { 
-    iDestruct (map_valid with "own_abs own_pod") as %Hlookup.
-    iPureIntro; exact Hlookup.
-  }
+  { iDestruct (map_valid with "own_abs own_pod") as %Hlookup. iPureIntro; exact Hlookup. }
+  iAssert (⌜ children !! parent_key = Some owned_child_keys ⌝%I) with "[own_children own_child_keys]" as "%parent_key_in_children".
+  { iDestruct (map_valid with "own_children own_child_keys") as %Hlookup. iPureIntro; exact Hlookup. }
+  iAssert (⌜ children !! key = Some owned_grandchild_keys ⌝%I) with "[own_children own_grandchild_keys]" as "%key_in_children".
+  { iDestruct (map_valid with "own_children own_grandchild_keys") as %Hlookup. iPureIntro; exact Hlookup. }
   iAssert (⌜ ∃ obj, phys_state !! key = Some obj ⌝%I) with "[phys_abs_rep]" as "%key_in_phys".
   {
     iDestruct (big_sepM2_lookup_r with "phys_abs_rep") as (obj key_in_phys) "_".
@@ -347,13 +372,13 @@ Proof.
   iDestruct (big_sepM2_split_singleton _ key _ _ phys_state abs_state key_in_phys key_in_abs with "phys_abs_rep") as "[k_rep other_rep]".
   destruct decide_kind_is_pod with (KKey.Kind' key) as [kind_is_pod kind_is_not_replicaset].
   { done. }
-  rewrite kind_is_pod.
-  iDestruct "k_rep" as "(%ptr & %rs0 & rs_rep)". iNamed "rs_rep".
+  iAssert (∃ (ptr: loc) (pod: v1.Pod.t), pod_rep key obj (KObject.Pod owned_pod) ptr pod)%I 
+  with "[k_rep]" as "(%ptr & %pod & pod_rep)".
+  { unfold obj_rep. rewrite kind_is_pod. done. }
+  iNamed "pod_rep".
   inversion abs_v_is_pod as [Heq]. symmetry in Heq. subst. clear abs_v_is_pod.
   wp_apply (wp_map_get with "[$own_phys]"). iIntros "own_phys". wp_auto.
   rewrite /is_Some key_in_phys. wp_auto.
-  destruct (pod_ptr_implements_v1_object (interface.mk (ptrT.id v1.Pod.id) (# ptr)) ptr) as [o [interface_is_object object_is_ptr]].
-  { done. }
   wp_apply wp_Accessor.
   { done. }
   iIntros (ret err) "(-> & ->)". wp_auto.
@@ -367,34 +392,298 @@ Proof.
   - wp_apply (wp_GetDeletionTimestamp with "[$HObjectMeta]").
     iIntros (deletion_timestamp) "(-> & HObjectMeta)". wp_auto.
     wp_if_destruct.
-    + wp_apply v1.wp_Now. iIntros (time) "_". wp_auto.
+    + wp_apply v1.wp_Now.
+      iIntros (time) "_". wp_auto.
       wp_apply (wp_SetDeletionTimestamp with "[$HObjectMeta]").
-      iIntros (meta') "(-> & HObjectMeta)". wp_auto.
+      iIntros (meta') "(-> & HObjectMeta)". wp_auto. wp_bind.
       wp_apply wp_globals_get.
-      (* TODO: handle resource version counter overflow *)
-      wp_apply wp_globals_get. wp_apply wp_globals_get.
+      (* TODO: fix the resource version counter overflow in the Go code *)
+      wp_apply wp_globals_get. wp_bind. wp_apply wp_globals_get.
       wp_apply wp_FormatInt. iIntros (rv_str) "_". wp_auto.
       wp_apply (wp_SetResourceVersion with "[$HObjectMeta]").
       iIntros (meta') "(-> & HObjectMeta)". wp_auto.
-      wp_apply wp_globals_get.
-      wp_apply (wp_map_insert with "[$own_phys]").
-      iIntros "own_phys". wp_auto.
       iDestruct (struct_fields_combine (v:=v1.Pod.mk _ _ _ _)
-        with "[$HTypeMeta $HObjectMeta $HSpec $HStatus]") as "new_pod_ptr". simpl.
-      admit.
-    + wp_apply wp_globals_get.
-      wp_apply (wp_map_insert with "[$own_phys]").
-      iIntros "own_phys". wp_auto.
-      iDestruct (struct_fields_combine (V:=v1.Pod.t)
-        with "[$HTypeMeta $HObjectMeta $HSpec $HStatus]") as "pod_ptr".
-      admit.
+        with "[$HTypeMeta $HObjectMeta $HSpec $HStatus]") as "pod_ptr". simpl.
+      iDestruct (rename_pod with "pod_ptr") as "(%updated_pod & pod_ptr & %updated_pod_eq)".
+      iMod (auth_map.map_update _ _ (KObject.Pod updated_pod) with "own_abs own_pod")
+        as "[own_abs own_pod]".
+      iAssert (state_rep phys_state (<[key:=KObject.Pod updated_pod]> abs_state) %I)
+      with "[pod_ptr other_rep pod_nn_well_formed]" as "phys_abs_rep".
+      {
+        assert (delete key abs_state = delete key (<[key:=KObject.Pod updated_pod]> abs_state)) as ->.
+        { rewrite delete_insert_eq. reflexivity. }
+        iAssert (pod_nn_well_formed updated_pod (KKey.Namespace' key) (KKey.Name' key)%I)
+        with "[pod_nn_well_formed]" as "pod_nn_well_formed".
+        {
+          iNamed "pod_nn_well_formed".
+          unfold pod_nn_well_formed. unfold pod_well_formed. unfold object_meta_well_formed.
+          subst updated_pod. simpl. iFrame. done.
+        }
+        iAssert (obj_rep key (interface.mk (ptrT.id v1.Pod.id) (# ptr)) (KObject.Pod updated_pod)%I)
+        with "[pod_ptr pod_nn_well_formed]" as "k_rep".
+        { unfold obj_rep. rewrite kind_is_pod. iExists ptr, updated_pod. iFrame. done. }
+        assert ((<[key:=KObject.Pod updated_pod]> abs_state) !! key = Some (KObject.Pod updated_pod)) as key_in_new_abs.
+        { rewrite lookup_insert. destruct (decide (key = key)) as [|Hcontra]; [reflexivity | contradiction]. }
+        iApply (big_sepM2_split_singleton _ key _ (KObject.Pod updated_pod) phys_state (<[key:=KObject.Pod updated_pod]> abs_state)
+          key_in_phys key_in_new_abs with "[k_rep other_rep]").
+        iFrame.
+      }
+      iAssert (kubernetes_state_consistent (<[key:=KObject.Pod updated_pod]> abs_state) children fresh_keys %I)
+      with "[consistent]"  as "consistent".
+      {
+        iNamed "consistent".
+        assert (parent_key ≠ key) as parent_neq_key.
+        { specialize (no_self_parenting parent_key owned_child_keys key parent_key_in_children pod_is_child). done. }
+        assert (dom (<[key:=KObject.Pod updated_pod]> abs_state) = dom abs_state) as abs_dom_simpl.
+        {
+          rewrite dom_insert_L.
+          assert ({[key]} ∪ dom abs_state = dom abs_state) as union_eq.
+          { set_solver. }
+          rewrite union_eq.
+          reflexivity.
+        }
+        assert ((extract_kobject_metadata (KObject.Pod updated_pod)).(v1.ObjectMeta.OwnerReferences') = (extract_kobject_metadata (KObject.Pod owned_pod)).(v1.ObjectMeta.OwnerReferences'))
+        as updated_pod_owner_references_eq.
+        { simpl. subst updated_pod. simpl. reflexivity. }
+        assert ((extract_kobject_metadata (KObject.Pod updated_pod)).(v1.ObjectMeta.UID') = (extract_kobject_metadata (KObject.Pod owned_pod)).(v1.ObjectMeta.UID'))
+        as updated_pod_uid_eq.
+        { simpl. subst updated_pod. simpl. reflexivity. }
+        iSplitR; [|iSplitR; [|iSplitR; [|iSplitR; [|iSplitR; [|iSplitR; [|iSplitL "children_point_to_parent"]]]]]].
+        { iPureIntro. set_solver. }
+        { iPureIntro. intros k s Hlookup. specialize (children_exist k s Hlookup). rewrite dom_insert_L. set_solver. }
+        { iPureIntro. apply parents_children_same_namespace. }
+        { iPureIntro. apply no_self_parenting. }
+        { iPureIntro. apply children_disjoint. }
+        { iPureIntro. rewrite dom_insert_L. set_solver. }
+        {
+          iIntros (k s parent child_key child) "(%Hlookup_children & %Hlookup_child & %Hlookup_parent & %Hchild_in_s)".
+          rewrite lookup_insert_Some in Hlookup_child.
+          rewrite lookup_insert_Some in Hlookup_parent.
+          destruct Hlookup_child as [(Heq_child & Hchild_eq) | (Hneq_child & Hlookup_child)];
+          destruct Hlookup_parent as [(Heq_parent & Hparent_eq) | (Hneq_parent & Hlookup_parent)].
+          - subst child_key k child parent.
+            exfalso.
+            apply (no_self_parenting key s key Hlookup_children Hchild_in_s).
+            reflexivity.
+          - subst child_key child.
+            rewrite updated_pod_owner_references_eq.
+            iApply "children_point_to_parent". done.
+          - subst k parent.
+            rewrite updated_pod_uid_eq.
+            iApply "children_point_to_parent". done.
+          - iApply ("children_point_to_parent" $! k s parent child_key child).
+            iPureIntro. done.
+        }
+        iIntros (k s parent child_key child) "[(%Hlookup_children & %Hlookup_child & %Hlookup_parent) Hmeta]".
+        rewrite lookup_insert_Some in Hlookup_child.
+        rewrite lookup_insert_Some in Hlookup_parent.
+        destruct Hlookup_child as [(Heq_child & Hchild_eq) | (Hneq_child & Hlookup_child)];
+        destruct Hlookup_parent as [(Heq_parent & Hparent_eq) | (Hneq_parent & Hlookup_parent)].
+        - subst child_key k child parent.
+          rewrite updated_pod_owner_references_eq.
+          rewrite updated_pod_uid_eq.
+          iDestruct ("only_children_point_to_parent" $! key s (KObject.Pod owned_pod) key (KObject.Pod owned_pod)
+            with "[Hmeta]") as "%Hkey_in_s".
+          { iFrame "Hmeta". iPureIntro. split; [|split]; assumption. }
+          exfalso.
+          apply (no_self_parenting key s key Hlookup_children Hkey_in_s).
+          reflexivity.
+        - subst child_key child.
+          rewrite updated_pod_owner_references_eq.
+          iApply ("only_children_point_to_parent" $! k s parent key (KObject.Pod owned_pod) with "[Hmeta]").
+          iFrame "Hmeta". iPureIntro. split; [|split]; assumption.
+        - subst k parent.
+          rewrite updated_pod_uid_eq.
+          iApply ("only_children_point_to_parent" $! key s (KObject.Pod owned_pod) child_key child with "[Hmeta]").
+          iFrame "Hmeta". iPureIntro. split; [|split]; assumption.
+        - iApply ("only_children_point_to_parent" $! k s parent child_key child with "[Hmeta]").
+          iFrame "Hmeta". iPureIntro. split; [|split]; assumption.
+      }
+      wp_apply (wp_Mutex__Unlock _ (is_kubernetes_state_inner γ_state γ_children γ_fresh_keys)
+      with "[$own_Mutex state_m_addr state_uc_addr state_rvc_addr own_phys own_abs phys_abs_rep own_children own_fresh_keys consistent]").
+      { iFrame. done. }
+      iApply "HΦ". iFrame. iSplitR; [done|]. iLeft. iFrame.
+      iAssert (⌜ now_ptr ≠ null ⌝%I) with "[now]" as "%now_ptr_not_null".
+      { by iDestruct (typed_pointsto_not_null with "now") as %?. }
+      iPureIntro. subst updated_pod. done.
+    + iDestruct (struct_fields_combine (V:=v1.Pod.t) with "[$HTypeMeta $HObjectMeta $HSpec $HStatus]") as "pod_ptr".
+      iAssert (state_rep phys_state abs_state %I) with "[pod_ptr other_rep pod_nn_well_formed]" as "phys_abs_rep".
+      {
+        iApply big_sepM2_split_singleton; [done | done|]. iFrame. unfold obj_rep. rewrite kind_is_pod.
+        iExists ptr, owned_pod. iFrame. done.
+      }
+      wp_apply (wp_Mutex__Unlock _ (is_kubernetes_state_inner γ_state γ_children γ_fresh_keys)
+        with "[$own_Mutex state_m_addr state_uc_addr state_rvc_addr own_phys own_abs phys_abs_rep own_children own_fresh_keys consistent]").
+      { iFrame. done. }
+      iApply "HΦ". iSplitR; [done|]. iLeft. iFrame. done.
   - wp_apply wp_globals_get.
     wp_apply (wp_map_delete with "[$own_phys]").
     iIntros "own_phys". wp_auto.
     iDestruct (struct_fields_combine (V:=v1.Pod.t)
-        with "[$HTypeMeta $HObjectMeta $HSpec $HStatus]") as "pod_ptr".
-    admit.
-Admitted.
+      with "[$HTypeMeta $HObjectMeta $HSpec $HStatus]") as "pod_ptr".
+    iMod (auth_map.map_delete with "own_pod own_abs") as "own_abs".
+    iMod (auth_map.map_update _ _ (owned_child_keys ∖ {[key]}) with "own_children own_child_keys")
+      as "[own_children own_child_keys]".
+    iMod (auth_map.map_delete with "own_grandchild_keys own_children") as "own_children".
+    iAssert (state_rep (delete key phys_state) (delete key abs_state) %I) with "[other_rep]" as "phys_abs_rep".
+    { done. }
+    iAssert (kubernetes_state_consistent (delete key abs_state) (delete key (<[parent_key:=owned_child_keys ∖ {[key]}]> children)) fresh_keys %I)
+    with "[consistent]"  as "consistent".
+    {
+      iNamed "consistent".
+      assert (parent_key ≠ key) as parent_neq_key.
+      { specialize (no_self_parenting parent_key owned_child_keys key parent_key_in_children pod_is_child). done. }
+      assert (dom (delete key (<[parent_key:=owned_child_keys ∖ {[key]}]> children)) = dom (delete key children) )
+      as children_dom_simpl.
+      {
+        assert (key ≠ parent_key) as key_neq_parent by (symmetry; exact parent_neq_key).
+        rewrite !dom_delete_L dom_insert_L.
+        assert (parent_key ∈ dom children) as parent_in_children_dom.
+        { apply elem_of_dom. exists owned_child_keys. exact parent_key_in_children. }
+        assert ({[parent_key]} ∪ dom children = dom children) as union_eq.
+        { set_solver. }
+        rewrite union_eq.
+        reflexivity.
+      }
+      iSplitR; [|iSplitR; [|iSplitR; [|iSplitR; [|iSplitR; [|iSplitR; [|iSplitL "children_point_to_parent"]]]]]].
+      { iPureIntro. set_solver. }
+      {
+        iPureIntro.
+        intros k s Hlookup.
+        rewrite lookup_delete_Some in Hlookup.
+        destruct Hlookup as (Hk_neq_key & Hlookup).
+        rewrite lookup_insert_Some in Hlookup.
+        destruct Hlookup as [(Hk_eq & Hs_eq) | (Hk_neq_parent & Hlookup)].
+        - assert (owned_child_keys ⊆ dom abs_state) as owned_children_in_abs.
+          { apply children_exist with (k := parent_key). exact parent_key_in_children. }
+          subst k s.
+          rewrite dom_delete_L.
+          set_solver.
+        - rewrite dom_delete_L.
+          assert (s ⊆ dom abs_state) as s_in_abs.
+          { apply children_exist with (k := k). exact Hlookup. }
+          assert (s ## owned_child_keys) as s_disj_owned.
+          {
+            destruct (decide (k = parent_key)) as [Heq | Hneq].
+            - subst k. congruence.
+            - apply children_disjoint with (k1 := k) (k2 := parent_key); assumption.
+          }
+          assert (key ∉ s) as key_not_in_s.
+          {
+            intros Hcontra.
+            assert (key ∈ owned_child_keys) by exact pod_is_child.
+            set_solver.
+          }
+          set_solver.
+      }
+      {
+        iPureIntro.
+        intros k s child_key Hlookup Hchild_in_s.
+        rewrite lookup_delete_Some in Hlookup.
+        destruct Hlookup as (Hk_neq_key & Hlookup).
+        rewrite lookup_insert_Some in Hlookup.
+        destruct Hlookup as [(Hk_eq & Hs_eq) | (Hk_neq_parent & Hlookup)].
+        - subst k s.
+          assert (child_key ∈ owned_child_keys) as child_in_owned.
+          { set_solver. }
+          apply parents_children_same_namespace with (k := parent_key) (s := owned_child_keys).
+          + exact parent_key_in_children.
+          + exact child_in_owned.
+        - apply parents_children_same_namespace with (k := k) (s := s).
+          + exact Hlookup.
+          + exact Hchild_in_s.
+      }
+      {
+        iPureIntro.
+        intros k s child_key Hlookup Hchild_in_s.
+        rewrite lookup_delete_Some in Hlookup.
+        destruct Hlookup as (Hk_neq_key & Hlookup).
+        rewrite lookup_insert_Some in Hlookup.
+        destruct Hlookup as [(Hk_eq & Hs_eq) | (Hk_neq_parent & Hlookup)].
+        - subst k s.
+          assert (child_key ∈ owned_child_keys) as child_in_owned.
+          { set_solver. }
+          apply no_self_parenting with (k := parent_key) (s := owned_child_keys).
+          + exact parent_key_in_children.
+          + exact child_in_owned.
+        - apply no_self_parenting with (k := k) (s := s).
+          + exact Hlookup.
+          + exact Hchild_in_s.
+      }
+      {
+        iPureIntro.
+        intros k1 s1 k2 s2 Hlookup1 Hlookup2.
+        rewrite lookup_delete_Some in Hlookup1.
+        rewrite lookup_delete_Some in Hlookup2.
+        destruct Hlookup1 as (Hk1_neq_key & Hlookup1).
+        destruct Hlookup2 as (Hk2_neq_key & Hlookup2).
+        rewrite lookup_insert_Some in Hlookup1.
+        rewrite lookup_insert_Some in Hlookup2.
+        destruct Hlookup1 as [(Hk1_eq & Hs1_eq) | (Hk1_neq_parent & Hlookup1)];
+        destruct Hlookup2 as [(Hk2_eq & Hs2_eq) | (Hk2_neq_parent & Hlookup2)].
+        - subst k1 k2 s1 s2.
+          assert (owned_child_keys ## owned_child_keys) as disj_self.
+          { apply children_disjoint with (k1 := parent_key) (k2 := parent_key); assumption. }
+          set_solver.
+        - subst k1 s1.
+          assert (owned_child_keys ## s2) as disj_orig.
+          { apply children_disjoint with (k1 := parent_key) (k2 := k2); assumption. }
+          set_solver.
+        - subst k2 s2.
+          assert (s1 ## owned_child_keys) as disj_orig.
+          { apply children_disjoint with (k1 := k1) (k2 := parent_key); assumption. }
+          set_solver.
+        - apply children_disjoint with (k1 := k1) (k2 := k2); assumption.
+      }
+      { iPureIntro. rewrite dom_delete_L. set_solver. }
+      {
+        iIntros (k s parent child_key child) "(%Hchildren_lookup & %Hchild_lookup & %Hparent_lookup & %Hchild_in_s)".
+        rewrite lookup_delete_Some in Hchildren_lookup.
+        destruct Hchildren_lookup as (Hk_neq_key, Hchildren_lookup).
+        rewrite lookup_delete_Some in Hchild_lookup.
+        destruct Hchild_lookup as (Hchild_key_neq_key, Hchild_lookup).
+        rewrite lookup_delete_Some in Hparent_lookup.
+        destruct Hparent_lookup as (Hk_neq_key', Hparent_lookup).
+        rewrite lookup_insert_Some in Hchildren_lookup.
+        destruct Hchildren_lookup as [(Hk_eq, Hs_eq) | (Hk_neq_parent, Hchildren_lookup)].
+        - subst k s.
+          assert (child_key ∈ owned_child_keys) as child_in_owned.
+          { set_solver. }
+          iApply ("children_point_to_parent" $! parent_key owned_child_keys parent child_key child).
+          iPureIntro.
+          split; [|split; [|split]]; assumption.
+        - iApply ("children_point_to_parent" $! k s parent child_key child).
+          iPureIntro.
+          split; [|split; [|split]]; assumption.
+      }
+      iIntros (k s parent child_key child) "[(%Hchildren_lookup & %Hchild_lookup & %Hparent_lookup) Hmeta]".
+      rewrite lookup_delete_Some in Hchildren_lookup.
+      destruct Hchildren_lookup as (Hk_neq_key, Hchildren_lookup).
+      rewrite lookup_delete_Some in Hchild_lookup.
+      destruct Hchild_lookup as (Hchild_key_neq_key, Hchild_lookup).
+      rewrite lookup_delete_Some in Hparent_lookup.
+      destruct Hparent_lookup as (Hk_neq_key', Hparent_lookup).
+      rewrite lookup_insert_Some in Hchildren_lookup.
+      destruct Hchildren_lookup as [(Hk_eq, Hs_eq) | (Hk_neq_parent, Hchildren_lookup)].
+      - subst k s.
+        iDestruct ("only_children_point_to_parent" $! parent_key owned_child_keys parent child_key child
+          with "[Hmeta]") as "%Hchild_in_owned".
+        { iFrame "Hmeta". iPureIntro. split; [|split]; assumption. }
+        iPureIntro.
+        set_solver.
+      - iDestruct ("only_children_point_to_parent" $! k s parent child_key child
+          with "[Hmeta]") as "%Hchild_in_s".
+        { iFrame "Hmeta". iPureIntro. split; [|split]; assumption. }
+        iPureIntro.
+        exact Hchild_in_s.
+    }
+    wp_apply (wp_Mutex__Unlock _ (is_kubernetes_state_inner γ_state γ_children γ_fresh_keys)
+      with "[$own_Mutex state_m_addr state_uc_addr state_rvc_addr own_phys own_abs phys_abs_rep own_children own_fresh_keys consistent]").
+    { iFrame. done. }
+    iApply "HΦ". iFrame. done.
+    Unshelve.
+    done.
+Qed.
 
 Lemma wp_PodDelete_ptsto_mut key γ_state γ_children γ_fresh_keys owned_pod parent_key owned_child_keys:
   {{{ is_pkg_init apimodel ∗
@@ -458,7 +747,7 @@ Proof.
   iDestruct (big_sepM2_lookup_acc _ _ _ _ _ _ key_in_phys key_in_abs with "phys_abs_rep") as "[k_rep other_rep]".
   destruct decide_kind_is_replicaset with (KKey.Kind' key) as [kind_is_replicaset kind_is_not_pod].
   { done. }
-  rewrite kind_is_replicaset kind_is_not_pod.
+  unfold obj_rep. rewrite kind_is_replicaset kind_is_not_pod.
   iDestruct "k_rep" as "(%ptr & %rs0 & rs_rep)". iNamed "rs_rep".
   inversion abs_v_is_rs as [Heq]. symmetry in Heq. subst. clear abs_v_is_rs.
   wp_apply (wp_map_get with "[$own_phys]"). iIntros "own_phys". wp_auto.
