src/proof/k8s_io/apimachinery/pkg/api/meta.v
@@ -5,16 +5,19 @@ From proof Require Import prelude empty_ffi.
 Section proof.
 Context `{hG: !heapGS Σ} {go_ctx: GoContext}.
 
-Lemma wp_Accessor i (o: v1.Object.t):
+(* FIXME: this spec is wrong because o's value should be a Pod pointer. will fix it after Goose has better support for
+  interface method dispatch *)
+Lemma wp_Accessor i ptr:
   {{{ is_pkg_init code.k8s_io.apimachinery.pkg.api.meta.meta ∗
-      "%i_is_Object" ∷ ⌜i = interface.mk v1.Object.id (# o)⌝
+      ⌜i = interface.mk (ptrT.id v1.Pod.id) (# ptr)⌝
   }}}
     @! meta.Accessor #i
-  {{{ ret (err: error.t), RET (#ret, #err);
-      ⌜ ret = o ⌝ ∗ ⌜ err = interface.nil ⌝
+  {{{ o (err: error.t), RET (#o, #err);
+      ⌜ o = interface.mk (ptrT.id v1.ObjectMeta.id) #(struct.field_ref_f v1.Pod "ObjectMeta" ptr) ⌝ ∗
+      ⌜ err = interface.nil ⌝
   }}}.
 Proof.
-  wp_start as "H". iNamed "H". wp_auto. subst.
+  (* wp_start as "H". iNamed "H". wp_auto. subst.
   unshelve wp_apply wp_interface_checked_type_assert; try tc_solve.
   { iPureIntro. intros Object_id. exists o. done. }
   iIntros (y ok) "%if_ok".
@@ -23,6 +26,7 @@ Proof.
   subst ok. inversion if_ok.
   apply (inj to_val) in H0. subst o.
   wp_auto. iApply "HΦ". done.
-Qed.
+Qed. *)
+Admitted.
 
 End proof.
